src/equations_common.ml
@@ -57,14 +57,20 @@ let check_type env evd t =
   ignore(Typing.sort_of env (ref evd) t)
       
 let typecheck_rel_context env evd ctx =
-  let _ =
-    List.fold_right
-      (fun (na, b, t as rel) env ->
-	 check_type env evd t;
-	 Option.iter (fun c -> check_term env evd c t) b;
-	 push_rel rel env)
-      ctx env
-  in ()
+  try
+    let _ =
+      List.fold_right
+        (fun (na, b, t as rel) env ->
+	  check_type env evd t;
+	  Option.iter (fun c -> check_term env evd c t) b;
+	  push_rel rel env)
+        ctx env
+    in ()
+  with e ->
+    Printf.eprintf "Exception while typechecking context %s : %s\n"
+                   (Pp.string_of_ppcmds (print_rel_context (push_rel_context ctx env)))
+                   (Printexc.to_string e);
+    raise e
 
 
 let new_untyped_evar () =
@@ -228,27 +234,28 @@ let get_one () = (!logic).logic_one
 let get_one_prf () = (!logic).logic_one_val
 let get_zero () = (!logic).logic_zero
 
-let mkapp evdref t args =
-  let evd, c = Evd.fresh_global (Global.env ()) !evdref (Lazy.force t) in
+let mkapp env evdref t args =
+  let evd, c = Evd.fresh_global env !evdref (Lazy.force t) in
   let _ = evdref := evd in
     mkApp (c, args)
 
-let refresh_universes_strict evd t = 
-  let evd', t' = Evarsolve.refresh_universes (Some true) (Global.env()) !evd t in
+let refresh_universes_strict env evd t = 
+  let evd', t' = Evarsolve.refresh_universes (Some true) env !evd t in
     evd := evd'; t'
 
-let mkEq evd t x y = 
-  mkapp evd (get_eq ()) [| refresh_universes_strict evd t; x; y |]
+let mkEq env evd t x y = 
+  mkapp env evd (get_eq ()) [| refresh_universes_strict env evd t; x; y |]
     
-let mkRefl evd t x = 
-  mkapp evd (get_eq_refl ()) [| refresh_universes_strict evd t; x |]
+let mkRefl env evd t x = 
+  mkapp env evd (get_eq_refl ()) [| refresh_universes_strict env evd t; x |]
 
-let mkHEq evd t x u y =
-  mkapp evd coq_heq [| refresh_universes_strict evd t; x; refresh_universes_strict evd u; y |]
+let mkHEq env evd t x u y =
+  mkapp env evd coq_heq [| refresh_universes_strict env evd t; x;
+                           refresh_universes_strict env evd u; y |]
     
-let mkHRefl evd t x =
-  mkapp evd coq_heq_refl
-    [| refresh_universes_strict evd t; x |]
+let mkHRefl env evd t x =
+  mkapp env evd coq_heq_refl
+    [| refresh_universes_strict env evd t; x |]
 
 let dummy_loc = Loc.dummy_loc 
 type 'a located = 'a Loc.located
